cedar-lean/Cedar/SymCCOpt/Verifier.lean
@@ -1,0 +1,141 @@
+/-
+ Copyright Cedar Contributors
+
+ Licensed under the Apache License, Version 2.0 (the "License");
+ you may not use this file except in compliance with the License.
+ You may obtain a copy of the License at
+
+      https://www.apache.org/licenses/LICENSE-2.0
+
+ Unless required by applicable law or agreed to in writing, software
+ distributed under the License is distributed on an "AS IS" BASIS,
+ WITHOUT WARRANTIES OR CONDITIONS OF ANY KIND, either express or implied.
+ See the License for the specific language governing permissions and
+ limitations under the License.
+-/
+
+import Cedar.SymCC.Verifier
+import Cedar.SymCCOpt.CompiledPolicies
+import Cedar.SymCCOpt.Enforcer
+
+/-!
+This file contains versions of the functions in `SymCC/Verifier.lean` that
+operate on compiled policies (from `SymCCOpt/CompiledPolicies.lean`).
+Unlike the unoptimized functions in `SymCC/Verifier.lean`, the functions in this
+file do not need to call the symbolic compiler.
+-/
+
+namespace Cedar.SymCC
+
+open Cedar.Spec Factory
+
+/--
+Returns asserts that are unsatisfiable iff the evaluation of `p`, represented
+as a `Term` of type .option .bool, satisfies `φ` on all inputs drawn from the
+`εnv` that `p` was compiled for.
+
+See also `verifyNeverErrorsOpt`.
+-/
+def verifyEvaluateOpt (φ : Term → Term) (p : CompiledPolicy) : Asserts :=
+  -- As an optimization here in `SymCCOpt`:
+  -- Our callers only pass relatively simple functions as `φ`.
+  -- We expect that `enforceCompiledPolicy` is much more expensive to compute than `φ`.
+  -- So, we first compute the assert involving `φ`. If that is constant-false, we
+  -- can just return constant-false and not compute `enforceCompiledPolicy`; the
+  -- resulting asserts are equivalent.
+  match not (φ p.term) with
+  | .prim (.bool false) => [false]
+  | assert => (enforceCompiledPolicy p).elts ++ [assert]
+
+/--
+Returns asserts that are unsatisfiable iff the authorization decisions produced
+by `ps₁` and `ps₂`, represented as `Term`s of type .bool, satisfy `φ` on all
+inputs drawn from the `εnv` that the policysets were compiled for.
+(Caller guarantees that `ps₁` and `ps₂` were compiled for the same `εnv`.)
+
+See also `verifyAlwaysAllowsOpt`, `verifyAlwaysDeniesOpt`, `verifyImpliesOpt`,
+`verifyEquivalentOpt`, and `verifyDisjointOpt`.
+-/
+def verifyIsAuthorizedOpt (φ : Term → Term → Term) (ps₁ ps₂ : CompiledPolicies) : Asserts :=
+  assert! ps₁.εnv = ps₂.εnv
+  -- As an optimization here in `SymCCOpt`:
+  -- Our callers only pass relatively simple functions as `φ`.
+  -- We expect that `enforcePairCompiledPolicies` is much more expensive to compute than `φ`.
+  -- So, we first compute the assert involving `φ`. If that is constant-false,
+  -- we can just return constant-false and not compute
+  -- `enforcePairCompiledPolicies`; the resulting asserts are equivalent.
+  match not (φ ps₁.term ps₂.term) with
+  | .prim (.bool false) => [false]
+  | assert => (enforcePairCompiledPolicies ps₁ ps₂).elts ++ [assert]
+
+/--
+Returns asserts that are unsatisfiable iff `p` does not error on any input in
+the `εnv` it was compiled for. If the asserts are satisfiable, then there is
+some input in `εnv` on which `p` errors.
+-/
+def verifyNeverErrorsOpt (p : CompiledPolicy) : Asserts :=
+  verifyEvaluateOpt isSome p
+
+/--
+Returns asserts that are unsatisfiable iff `p` matches all inputs in the `εnv`
+it was compiled for.  If the asserts are satisfiable, then there is some input
+in `εnv` which `p` doesn't match.
+-/
+def verifyAlwaysMatchesOpt (p : CompiledPolicy) : Asserts :=
+  verifyEvaluateOpt (eq · (⊙true)) p
+
+/--
+Returns asserts that are unsatisfiable iff `p` matches no inputs in `εnv`.
+If the asserts are satisfiable, then there is some input in `εnv` which `p`
+does match.
+-/
+def verifyNeverMatchesOpt (p : CompiledPolicy) : Asserts :=
+  verifyEvaluateOpt (λ t => not (eq t (⊙true))) p
+
+/--
+Returns asserts that are unsatisfiable iff the authorization decision of `ps₁`
+implies that of `ps₂` for every input in the `εnv` that the policysets were
+compiled for.
+(Caller guarantees that `ps₁` and `ps₂` were compiled for the same `εnv`.)
+In other words, every input allowed by `ps₁` is allowed by `ps₂`.
+-/
+def verifyImpliesOpt (ps₁ ps₂ : CompiledPolicies) : Asserts :=
+  verifyIsAuthorizedOpt implies ps₁ ps₂
+
+/--
+Returns asserts that are unsatisfiable iff `ps` allows all inputs in the `εnv`
+it was compiled for.
+-/
+def verifyAlwaysAllowsOpt (ps : CompiledPolicies) : Asserts :=
+  verifyImpliesOpt (CompiledPolicies.allowAll ps.εnv) ps
+
+/--
+Returns asserts that are unsatisfiable iff `ps` denies all inputs in the `εnv`
+it was compiled for.
+-/
+def verifyAlwaysDeniesOpt (ps : CompiledPolicies) : Asserts :=
+  verifyImpliesOpt ps (CompiledPolicies.denyAll ps.εnv)
+
+/--
+Returns asserts that are unsatisfiable iff `ps₁` and `ps₂` produce the same
+authorization decision on all inputs in the `εnv` that the policysets were
+compiled for.
+(Caller guarantees that `ps₁` and `ps₂` were compiled for the same `εnv`.)
+-/
+def verifyEquivalentOpt (ps₁ ps₂ : CompiledPolicies) : Asserts :=
+  verifyIsAuthorizedOpt eq ps₁ ps₂
+
+/--
+Returns asserts that are unsatisfiable iff there is no input in the `εnv` that
+is allowed by both `ps₁` and `ps₂`.
+(Caller guarantees that `ps₁` and `ps₂` were compiled for the same `εnv`.)
+This checks that the authorization semantics of `ps₁` and `ps₂` are disjoint.
+If this query is satisfiable, then there is at least one input in this `εnv` that
+is allowed by both `ps₁` and `ps₂`.
+-/
+def verifyDisjointOpt (ps₁ ps₂ : CompiledPolicies) : Asserts :=
+  verifyIsAuthorizedOpt disjoint ps₁ ps₂
+where
+  disjoint (t₁ t₂ : Term) := not (and t₁ t₂)
+
+end Cedar.SymCC
