cedar-lean/Cedar/Thm.lean
@@ -17,6 +17,7 @@
 import Cedar.Thm.Data
 import Cedar.Thm.Authorization
 import Cedar.Thm.PolicySlice
+import Cedar.Thm.SymCC.Opt
 import Cedar.Thm.Typechecking
 import Cedar.Thm.Validation
 import Cedar.Thm.WellTyped
