cedar-lean/Cedar/Thm/SymCC/Opt.lean
@@ -1,0 +1,1397 @@
+/-
+ Copyright Cedar Contributors
+
+ Licensed under the Apache License, Version 2.0 (the "License");
+ you may not use this file except in compliance with the License.
+ You may obtain a copy of the License at
+
+      https://www.apache.org/licenses/LICENSE-2.0
+
+ Unless required by applicable law or agreed to in writing, software
+ distributed under the License is distributed on an "AS IS" BASIS,
+ WITHOUT WARRANTIES OR CONDITIONS OF ANY KIND, either express or implied.
+ See the License for the specific language governing permissions and
+ limitations under the License.
+-/
+
+import Cedar.SymCC
+import Cedar.SymCCOpt
+import Cedar.Thm.Data.Control
+import Cedar.Thm.Data.Set
+import Cedar.Thm.SymCC.Authorizer
+import Cedar.Thm.SymCC.Opt.AllowDeny
+import Cedar.Thm.SymCC.Opt.Asserts
+import Cedar.Thm.SymCC.Opt.CompiledPolicies
+import Cedar.Thm.WellTypedVerification
+
+/-!
+Proofs that the optimized interface in SymCCOpt is equivalent to the unoptimized
+interface in SymCC.
+-/
+
+namespace Cedar.Thm
+
+open Cedar.Spec Cedar.SymCC
+
+/--
+This theorem covers the "happy path" -- showing that if optimized policy
+compilation succeeds, then `enforce` and `enforceCompiledPolicy` are equivalent.
+-/
+theorem enforceCompiledPolicy_eqv_enforce_ok {p wp : Policy} {cp : CompiledPolicy} {Γ : Validation.TypeEnv} :
+  CompiledPolicy.compile p Γ = .ok cp →
+  wellTypedPolicy p Γ = .ok wp →
+  enforce [wp.toExpr] (SymEnv.ofTypeEnv Γ) = enforceCompiledPolicy cp
+:= by
+  simp [enforce, enforceCompiledPolicy]
+  intro h₀ h₁
+  simp [
+    cp_compile_produces_the_right_env h₀,
+    cp_compile_produces_the_right_footprint h₀,
+    cp_compile_produces_the_right_acyclicity h₀,
+    compiled_policy_eq_wtp h₀ h₁,
+  ]
+  simp [footprints]
+  simp [Data.Set.make_make_eqv, List.Equiv, List.subset_def]
+  constructor
+  · intro t h₂
+    cases h₂
+    · left
+      rename_i h₂
+      replace ⟨t', h₂, ht⟩ := h₂ ; subst t ; rename Term => t
+      rw [Data.Set.in_list_iff_in_set] at *
+      rw [Data.Set.mem_mapUnion_iff_mem_exists] at h₂
+      replace ⟨s, hs, h₂⟩ := h₂
+      simp at hs ; subst s
+      simp [Data.Set.mem_map]
+      exists t
+    · right
+      rename_i h₂
+      simp [List.mem_mapUnion_iff_mem_exists] at *
+      replace ⟨s, hs, t', ht', h₂⟩ := h₂ ; subst t ; rename Term => t
+      simp [Data.Set.in_list_iff_in_set, Data.Set.mem_mapUnion_iff_mem_exists] at *
+      exists s
+      simp [hs]
+      exists t
+  · intro t h₂
+    cases h₂
+    · left
+      rename_i h₂
+      simp [Data.Set.in_list_iff_in_set, Data.Set.mem_map] at h₂
+      replace ⟨t', ht', h₂⟩ := h₂ ; subst t ; rename Term => t
+      exists t
+      simp [Data.Set.in_list_iff_in_set, Data.Set.mem_mapUnion_iff_mem_exists]
+      exact ht'
+    · right
+      rename_i h₂
+      rw [List.mem_mapUnion_iff_mem_exists] at *
+      simp only [List.mem_map] at *
+      replace ⟨s, hs, t', ht', h₂⟩ := h₂ ; subst t ; rename Term => t
+      exists s
+      rw [Data.Set.in_list_iff_in_set] at *
+      simp [Data.Set.mem_mapUnion_iff_mem_exists, hs]
+      exists t
+      simp [Data.Set.in_list_iff_in_set, Data.Set.mem_mapUnion_iff_mem_exists, ht']
+
+/--
+This theorem covers the "happy path" -- showing that if optimized policy
+compilation succeeds, then `enforce` and `enforcePairCompiledPolicies` are
+equivalent.
+-/
+theorem enforcePairCompiledPolicies_eqv_enforce_ok {ps₁ ps₂ wps₁ wps₂ : Policies} {cps₁ cps₂ : CompiledPolicies} {Γ : Validation.TypeEnv} :
+  CompiledPolicies.compile ps₁ Γ = .ok cps₁ →
+  CompiledPolicies.compile ps₂ Γ = .ok cps₂ →
+  wellTypedPolicies ps₁ Γ = .ok wps₁ →
+  wellTypedPolicies ps₂ Γ = .ok wps₂ →
+  enforce (wps₁.map Policy.toExpr ++ wps₂.map Policy.toExpr) (SymEnv.ofTypeEnv Γ) = enforcePairCompiledPolicies cps₁ cps₂
+:= by
+  simp [enforce, enforcePairCompiledPolicies]
+  intro hcps₁ hcps₂ hwps₁ hwps₂
+  simp [
+    cps_compile_produces_the_right_env hcps₁,
+    cps_compile_produces_the_right_env hcps₂,
+    cps_compile_produces_the_right_footprint hcps₁,
+    cps_compile_produces_the_right_footprint hcps₂,
+    cps_compile_produces_the_right_acyclicity hcps₁,
+    cps_compile_produces_the_right_acyclicity hcps₂,
+    compiled_policies_eq_wtps hcps₁ hwps₁,
+    compiled_policies_eq_wtps hcps₂ hwps₂,
+  ]
+  simp [footprints_append]
+  rw [Data.Set.make_make_eqv]
+  simp [List.Equiv, List.subset_def]
+  constructor
+  · intro t₁ h₁
+    cases h₁ <;> rename_i h₁
+    · replace ⟨t₂, h₁, htemp⟩ := h₁ ; subst t₁
+      simp [Data.Set.in_list_iff_in_set] at *
+      simp [footprints]
+      change t₂ ∈ _ ∪ _ at h₁
+      rw [Data.Set.mem_union_iff_mem_or] at h₁
+      cases h₁ <;> rename_i h₁
+      case' inl => left
+      case' inr => right ; left
+      all_goals {
+        simp [footprints] at h₁
+        rw [Data.Set.mem_mapUnion_iff_mem_exists] at h₁
+        replace ⟨x, h₁, h₂⟩ := h₁
+        simp [Data.Set.mem_map]
+        exists t₂
+        simp [Data.Set.mem_mapUnion_iff_mem_exists]
+        exists x
+        apply And.intro _ h₂
+        rw [List.mem_map] at h₁
+        exact h₁
+      }
+    · right ; right
+      simp [*]
+  · intro t₁ h₁
+    cases h₁ <;> rename_i h₁ <;> try (cases h₁ <;> rename_i h₁)
+    case right.inr.inr => right ; exact h₁
+    case' right.inl | right.inr.inl =>
+      left
+      simp [Data.Set.in_list_iff_in_set, Data.Set.mem_map] at h₁
+      replace ⟨t₂, h₁, htemp⟩ := h₁ ; subst t₁
+      simp [mem_footprints_iff] at h₁
+      replace ⟨x, ⟨p, hp, htemp⟩, h₁⟩ := h₁ ; subst x
+      exists t₂
+      simp [Data.Set.in_list_iff_in_set, HAppend.hAppend]
+      change t₂ ∈ _ ∪ _
+      rw [Data.Set.mem_union_iff_mem_or]
+    case' right.inl => left
+    case' right.inr.inl => right
+    all_goals {
+      simp [mem_footprints_iff]
+      exists p.toExpr
+      apply And.intro _ h₁
+      exists p
+    }
+
+/--
+This theorem covers the "happy path" -- showing that if optimized policy
+compilation succeeds, then `verifyEvaluate` and `verifyEvaluateOpt` are
+equivalent.
+-/
+theorem verifyEvaluateOpt_eqv_verifyEvaluate_ok {p wp : Policy} {cp : CompiledPolicy} {Γ : Validation.TypeEnv} {φ : Term → Term} :
+  CompiledPolicy.compile p Γ = .ok cp →
+  wellTypedPolicy p Γ = .ok wp →
+  verifyEvaluate φ wp (SymEnv.ofTypeEnv Γ) ~ .ok (verifyEvaluateOpt φ cp)
+:= by
+  simp [verifyEvaluate, verifyEvaluateOpt, ResultAssertsEquiv]
+  intro h₀ h₁
+  simp [enforceCompiledPolicy_eqv_enforce_ok h₀ h₁]
+  cases h₂ : compile wp.toExpr (SymEnv.ofTypeEnv Γ) <;> simp
+  case error e => simp_all [CompiledPolicy.compile, Except.mapError]
+  case ok t =>
+    have h₃ := (cp_compile_produces_the_right_term h₀ h₁).symm ; simp [h₂] at h₃ ; subst t
+    split <;> rename_i hnot
+    · apply Asserts.Equiv.constantFalse <;> simp [hnot]
+    · apply Asserts.Equiv.rfl
+
+/--
+This theorem covers the "happy path" -- showing that if optimized policy
+compilation succeeds, then `verifyIsAuthorized` and `verifyIsAuthorizedOpt` are
+equivalent.
+-/
+theorem verifyIsAuthorizedOpt_eqv_verifyIsAuthorized_ok {ps₁ ps₂ wps₁ wps₂ : Policies} {cps₁ cps₂ : CompiledPolicies} {Γ : Validation.TypeEnv} {φ : Term → Term → Term} :
+  CompiledPolicies.compile ps₁ Γ = .ok cps₁ →
+  CompiledPolicies.compile ps₂ Γ = .ok cps₂ →
+  wellTypedPolicies ps₁ Γ = .ok wps₁ →
+  wellTypedPolicies ps₂ Γ = .ok wps₂ →
+  verifyIsAuthorized φ wps₁ wps₂ (SymEnv.ofTypeEnv Γ) ~ .ok (verifyIsAuthorizedOpt φ cps₁ cps₂)
+:= by
+  simp [verifyIsAuthorized, verifyIsAuthorizedOpt, ResultAssertsEquiv]
+  intro hcps₁ hcps₂ hwps₁ hwps₂
+  simp [enforcePairCompiledPolicies_eqv_enforce_ok hcps₁ hcps₂ hwps₁ hwps₂]
+  have henvs : cps₁.εnv = cps₂.εnv := by
+    simp [cps_compile_produces_the_right_env hcps₁, cps_compile_produces_the_right_env hcps₂]
+  simp [henvs]
+  cases h₁ : SymCC.isAuthorized wps₁ (SymEnv.ofTypeEnv Γ) <;> simp
+  case error e => simp_all [CompiledPolicies.compile, SymCC.isAuthorized, SymCC.satisfiedPolicies, SymCC.compileWithEffect, Except.mapError]
+  case ok t =>
+    have h₃ := (cps_compile_produces_the_right_term hcps₁ hwps₁).symm ; simp [h₁] at h₃ ; subst t
+    cases h₂ : SymCC.isAuthorized wps₂ (SymEnv.ofTypeEnv Γ) <;> simp
+    case error e => simp_all [CompiledPolicies.compile, SymCC.isAuthorized, SymCC.satisfiedPolicies, SymCC.compileWithEffect, Except.mapError]
+    case ok t =>
+      have h₃ := (cps_compile_produces_the_right_term hcps₂ hwps₂).symm ; simp [h₂] at h₃ ; subst t
+      split <;> rename_i hnot
+      · apply Asserts.Equiv.constantFalse <;> simp [hnot]
+      · apply Asserts.Equiv.rfl
+
+/--
+This theorem covers the "happy path" -- showing that if optimized policy
+compilation succeeds, then `verifyNeverErrors` and `verifyNeverErrorsOpt` are
+equivalent.
+-/
+theorem verifyNeverErrorsOpt_eqv_verifyNeverErrors_ok {p wp : Policy} {cp : CompiledPolicy} {Γ : Validation.TypeEnv} :
+  CompiledPolicy.compile p Γ = .ok cp →
+  wellTypedPolicy p Γ = .ok wp →
+  verifyNeverErrors wp (SymEnv.ofTypeEnv Γ) ~ .ok (verifyNeverErrorsOpt cp)
+:= by
+  simp [verifyNeverErrors, verifyNeverErrorsOpt]
+  exact verifyEvaluateOpt_eqv_verifyEvaluate_ok
+
+/--
+This theorem covers the "happy path" -- showing that if optimized policy
+compilation succeeds, then `verifyAlwaysMatches` and `verifyAlwaysMatchesOpt` are
+equivalent.
+-/
+theorem verifyAlwaysMatchesOpt_eqv_verifyAlwaysMatches_ok {p wp : Policy} {cp : CompiledPolicy} {Γ : Validation.TypeEnv} :
+  CompiledPolicy.compile p Γ = .ok cp →
+  wellTypedPolicy p Γ = .ok wp →
+  verifyAlwaysMatches wp (SymEnv.ofTypeEnv Γ) ~ .ok (verifyAlwaysMatchesOpt cp)
+:= by
+  simp [verifyAlwaysMatches, verifyAlwaysMatchesOpt]
+  exact verifyEvaluateOpt_eqv_verifyEvaluate_ok
+
+/--
+This theorem covers the "happy path" -- showing that if optimized policy
+compilation succeeds, then `verifyNeverMatches` and `verifyNeverMatchesOpt` are
+equivalent.
+-/
+theorem verifyNeverMatchesOpt_eqv_verifyNeverMatches_ok {p wp : Policy} {cp : CompiledPolicy} {Γ : Validation.TypeEnv} :
+  CompiledPolicy.compile p Γ = .ok cp →
+  wellTypedPolicy p Γ = .ok wp →
+  verifyNeverMatches wp (SymEnv.ofTypeEnv Γ) ~ .ok (verifyNeverMatchesOpt cp)
+:= by
+  simp [verifyNeverMatches, verifyNeverMatchesOpt]
+  exact verifyEvaluateOpt_eqv_verifyEvaluate_ok
+
+/--
+This theorem covers the "happy path" -- showing that if optimized policy
+compilation succeeds, then `verifyImplies` and `verifyImpliesOpt` are
+equivalent.
+-/
+theorem verifyImpliesOpt_eqv_verifyImplies_ok {ps₁ ps₂ wps₁ wps₂ : Policies} {cps₁ cps₂ : CompiledPolicies} {Γ : Validation.TypeEnv} :
+  CompiledPolicies.compile ps₁ Γ = .ok cps₁ →
+  CompiledPolicies.compile ps₂ Γ = .ok cps₂ →
+  wellTypedPolicies ps₁ Γ = .ok wps₁ →
+  wellTypedPolicies ps₂ Γ = .ok wps₂ →
+  verifyImplies wps₁ wps₂ (SymEnv.ofTypeEnv Γ) ~ .ok (verifyImpliesOpt cps₁ cps₂)
+:= by
+  simp [verifyImplies, verifyImpliesOpt]
+  exact verifyIsAuthorizedOpt_eqv_verifyIsAuthorized_ok
+
+/--
+This theorem covers the "happy path" -- showing that if optimized policy
+compilation succeeds, then `verifyAlwaysAllows` and `verifyAlwaysAllowsOpt` are
+equivalent.
+-/
+theorem verifyAlwaysAllowsOpt_eqv_verifyAlwaysAllows_ok {ps wps : Policies} {cps : CompiledPolicies} {Γ : Validation.TypeEnv} :
+  CompiledPolicies.compile ps Γ = .ok cps →
+  wellTypedPolicies ps Γ = .ok wps →
+  verifyAlwaysAllows wps (SymEnv.ofTypeEnv Γ) ~ .ok (verifyAlwaysAllowsOpt cps)
+:= by
+  simp [verifyAlwaysAllows, verifyAlwaysAllowsOpt]
+  intro hcps hwps
+  apply verifyImpliesOpt_eqv_verifyImplies_ok _ hcps (wellTypedPolicies_allowAll Γ) hwps
+  simp [CompiledPolicies.compile, Except.mapError, do_eq_ok]
+  simp [wellTypedPolicies_allowAll, isAuthorized_allowAll]
+  simp [CompiledPolicies.allowAll, cps_compile_produces_the_right_env hcps]
+  simp [footprints_singleton]
+
+/--
+This theorem covers the "happy path" -- showing that if optimized policy
+compilation succeeds, then `verifyAlwaysAllows` and `verifyAlwaysAllowsOpt` are
+equivalent.
+-/
+theorem verifyAlwaysDeniesOpt_eqv_verifyAlwaysDenies_ok {ps wps : Policies} {cps : CompiledPolicies} {Γ : Validation.TypeEnv} :
+  CompiledPolicies.compile ps Γ = .ok cps →
+  wellTypedPolicies ps Γ = .ok wps →
+  verifyAlwaysDenies wps (SymEnv.ofTypeEnv Γ) ~ .ok (verifyAlwaysDeniesOpt cps)
+:= by
+  simp [verifyAlwaysDenies, verifyAlwaysDeniesOpt]
+  intro hcps hwps
+  apply verifyImpliesOpt_eqv_verifyImplies_ok hcps _ hwps _ (ps₂ := [])
+  simp [CompiledPolicies.compile, Except.mapError, do_eq_ok]
+  simp [wellTypedPolicies_empty, isAuthorized_empty]
+  simp [CompiledPolicies.denyAll, cps_compile_produces_the_right_env hcps]
+  simp [footprints_empty, EmptyCollection.emptyCollection, Data.Set.map_empty]
+  simp [wellTypedPolicies_empty]
+
+/--
+This theorem covers the "happy path" -- showing that if optimized policy
+compilation succeeds, then `verifyEquivalent` and `verifyEquivalentOpt` are
+equivalent.
+-/
+theorem verifyEquivalentOpt_eqv_verifyEquivalent_ok {ps₁ ps₂ wps₁ wps₂ : Policies} {cps₁ cps₂ : CompiledPolicies} {Γ : Validation.TypeEnv} :
+  CompiledPolicies.compile ps₁ Γ = .ok cps₁ →
+  CompiledPolicies.compile ps₂ Γ = .ok cps₂ →
+  wellTypedPolicies ps₁ Γ = .ok wps₁ →
+  wellTypedPolicies ps₂ Γ = .ok wps₂ →
+  verifyEquivalent wps₁ wps₂ (SymEnv.ofTypeEnv Γ) ~ .ok (verifyEquivalentOpt cps₁ cps₂)
+:= by
+  simp [verifyEquivalent, verifyEquivalentOpt]
+  exact verifyIsAuthorizedOpt_eqv_verifyIsAuthorized_ok
+
+/--
+This theorem covers the "happy path" -- showing that if optimized policy
+compilation succeeds, then `verifyDisjoint` and `verifyDisjointOpt` are
+equivalent.
+-/
+theorem verifyDisjointOpt_eqv_verifyDisjoint_ok {ps₁ ps₂ wps₁ wps₂ : Policies} {cps₁ cps₂ : CompiledPolicies} {Γ : Validation.TypeEnv} :
+  CompiledPolicies.compile ps₁ Γ = .ok cps₁ →
+  CompiledPolicies.compile ps₂ Γ = .ok cps₂ →
+  wellTypedPolicies ps₁ Γ = .ok wps₁ →
+  wellTypedPolicies ps₂ Γ = .ok wps₂ →
+  verifyDisjoint wps₁ wps₂ (SymEnv.ofTypeEnv Γ) ~ .ok (verifyDisjointOpt cps₁ cps₂)
+:= by
+  simp [verifyDisjoint, verifyDisjointOpt]
+  exact verifyIsAuthorizedOpt_eqv_verifyIsAuthorized_ok
+
+/--
+If `SymCC.satisfiedPolicies` fails, that must be because `SymCC.compile` failed
+with that error on some policy
+-/
+theorem satisfiedPolicies_eq_error {e : SymCC.Error} {effect : Effect} {ps : Policies} {εnv : SymEnv} :
+  SymCC.satisfiedPolicies effect ps εnv = .error e →
+  ∃ p ∈ ps, SymCC.compile p.toExpr εnv = .error e
+:= by
+  simp only [SymCC.satisfiedPolicies, do_error]
+  intro h
+  replace ⟨p, hp, h⟩ := List.filterMapM_error_implies_exists_error h
+  exists p ; apply And.intro hp
+  simp [compileWithEffect] at h
+  split at h
+  · simp [Functor.map, Except.map] at h
+    split at h <;> simp at h
+    subst h
+    assumption
+  · simp at h
+
+/--
+If `SymCC.isAuthorized` fails, that must be because `SymCC.compile` failed with
+that error on some policy
+-/
+theorem isAuthorized_eq_error {e : SymCC.Error} {ps : Policies} {εnv : SymEnv} :
+  SymCC.isAuthorized ps εnv = .error e →
+  ∃ p ∈ ps, SymCC.compile p.toExpr εnv = .error e
+:= by
+  simp [SymCC.isAuthorized]
+  cases h : SymCC.satisfiedPolicies .forbid ps εnv <;> simp
+  case error e' => intro _ ; subst e' ; exact satisfiedPolicies_eq_error h
+  case ok t => simp only [do_error] ; exact satisfiedPolicies_eq_error
+
+/--
+`CompiledPolicy.compile` succeeds iff `wellTypedPolicy` succeeds
+
+Note: `Γ.WellFormed` is technically only required for the reverse direction
+-/
+theorem compile_ok_iff_welltypedpolicy_ok {p : Policy} {Γ : Validation.TypeEnv} :
+  Γ.WellFormed → (
+  Except.isOk (CompiledPolicy.compile p Γ) ↔
+  Except.isOk (wellTypedPolicy p Γ)
+  )
+:= by
+  simp [Except.isOk, Except.toBool]
+  simp [CompiledPolicy.compile, Except.mapError]
+  cases h₀ : wellTypedPolicy p Γ <;> simp
+  case ok wp =>
+    intro hwf
+    have ⟨tx, htxwt, htx⟩ := wellTypedPolicy_ok_implies_well_typed_expr h₀
+    have ⟨t, ht, _⟩ := compile_well_typed hwf htxwt
+    simp_all
+
+/--
+`CompiledPolicies.compile` succeeds iff `wellTypedPolicies` succeeds
+
+Note: `Γ.WellFormed` is technically only required for the reverse direction
+-/
+theorem compile_ok_iff_welltypedpolicies_ok {ps : Policies} {Γ : Validation.TypeEnv} :
+  Γ.WellFormed → (
+  Except.isOk (CompiledPolicies.compile ps Γ) ↔
+  Except.isOk (wellTypedPolicies ps Γ)
+  )
+:= by
+  simp [Except.isOk, Except.toBool]
+  simp [CompiledPolicies.compile, Except.mapError]
+  cases hwp : wellTypedPolicies ps Γ <;> simp
+  case ok wps =>
+    intro hwf
+    split <;> simp
+    rename_i e h
+    simp [do_error] at h
+    split at h <;> simp at h
+    subst e
+    rename_i e h
+    simp [wellTypedPolicies] at hwp
+    replace ⟨wp, hwp', h⟩ := isAuthorized_eq_error h
+    replace ⟨p, hp, hwp⟩ := List.mapM_ok_implies_all_from_ok hwp wp hwp'
+    have ⟨tx, htxwt, htx⟩ := wellTypedPolicy_ok_implies_well_typed_expr hwp
+    have ⟨t, ht, _⟩ := compile_well_typed hwf htxwt
+    simp_all
+
+/--
+If `CompiledPolicy.compile` succeeds, then `wellTypedPolicy` succeeds
+
+Note: Can be proved without `Γ.WellFormed`
+-/
+theorem compile_ok_then_exists_wtp {p : Policy} {cp : CompiledPolicy} {Γ : Validation.TypeEnv} :
+  Γ.WellFormed →
+  CompiledPolicy.compile p Γ = .ok cp →
+  ∃ wp, wellTypedPolicy p Γ = .ok wp
+:= by
+  intro hwf h₀
+  have h₁ := (compile_ok_iff_welltypedpolicy_ok hwf).mp (by
+    simp [Except.isOk_iff_exists]
+    exists cp
+  )
+  simp [Except.isOk_iff_exists] at h₁
+  exact h₁
+
+/--
+If `CompiledPolicies.compile` succeeds, then `wellTypedPolicies` succeeds
+
+Note: Can be proved without `Γ.WellFormed`
+-/
+theorem compile_ok_then_exists_wtps {ps : Policies} {cps : CompiledPolicies} {Γ : Validation.TypeEnv} :
+  Γ.WellFormed →
+  CompiledPolicies.compile ps Γ = .ok cps →
+  ∃ wps, wellTypedPolicies ps Γ = .ok wps
+:= by
+  intro hwf h₀
+  have h₁ := (compile_ok_iff_welltypedpolicies_ok hwf).mp (by
+    simp [Except.isOk_iff_exists]
+    exists cps
+  )
+  simp [Except.isOk_iff_exists] at h₁
+  exact h₁
+
+/--
+This theorem covers the "happy path" -- showing that if optimized policy
+compilation succeeds, then `wellTypedPolicy` succeeds and `neverErrors?` and
+`neverErrorsOpt?` are equivalent.
+-/
+theorem neverErrorsOpt?_eqv_neverErrors?_ok {p : Policy} {cp : CompiledPolicy} {Γ : Validation.TypeEnv} :
+  Γ.WellFormed →
+  CompiledPolicy.compile p Γ = .ok cp →
+  ∃ wp,
+    wellTypedPolicy p Γ = .ok wp ∧
+    neverErrorsOpt? cp = neverErrors? wp (SymEnv.ofTypeEnv Γ)
+:= by
+  simp [neverErrors?, neverErrorsOpt?]
+  simp [sat?]
+  intro hwf h₀
+  have ⟨wp, h₁⟩ := compile_ok_then_exists_wtp hwf h₀
+  exists wp ; apply And.intro h₁
+  have ⟨asserts, h₂⟩ := verifyNeverErrors_is_ok hwf h₁
+  simp [h₂]
+  simp [cp_compile_produces_the_right_env h₀]
+  simp [compiled_policy_eq_wtp h₀ h₁]
+  have := verifyNeverErrorsOpt_eqv_verifyNeverErrors_ok h₀ h₁
+  simp [h₂, ResultAssertsEquiv] at this
+  exact Asserts.Equiv.satAsserts? [wp] _ (Asserts.Equiv.symm this)
+
+/--
+This theorem covers the "happy path" -- showing that if optimized policy
+compilation succeeds, then `wellTypedPolicy` succeeds and `alwaysMatches?` and
+`alwaysMatchesOpt?` are equivalent.
+-/
+theorem alwaysMatchesOpt?_eqv_alwaysMatches?_ok {p : Policy} {cp : CompiledPolicy} {Γ : Validation.TypeEnv} :
+  Γ.WellFormed →
+  CompiledPolicy.compile p Γ = .ok cp →
+  ∃ wp,
+    wellTypedPolicy p Γ = .ok wp ∧
+    alwaysMatchesOpt? cp = alwaysMatches? wp (SymEnv.ofTypeEnv Γ)
+:= by
+  simp [alwaysMatches?, alwaysMatchesOpt?]
+  simp [sat?]
+  intro hwf h₀
+  have ⟨wp, h₁⟩ := compile_ok_then_exists_wtp hwf h₀
+  exists wp ; apply And.intro h₁
+  have ⟨asserts, h₂⟩ := verifyAlwaysMatches_is_ok hwf h₁
+  simp [h₂]
+  simp [cp_compile_produces_the_right_env h₀]
+  simp [compiled_policy_eq_wtp h₀ h₁]
+  have := verifyAlwaysMatchesOpt_eqv_verifyAlwaysMatches_ok h₀ h₁
+  simp [h₂, ResultAssertsEquiv] at this
+  exact Asserts.Equiv.satAsserts? [wp] _ (Asserts.Equiv.symm this)
+
+/--
+This theorem covers the "happy path" -- showing that if optimized policy
+compilation succeeds, then `wellTypedPolicy` succeeds and `neverMatches?` and
+`neverMatchesOpt?` are equivalent.
+-/
+theorem neverMatchesOpt?_eqv_neverMatches?_ok {p : Policy} {cp : CompiledPolicy} {Γ : Validation.TypeEnv} :
+  Γ.WellFormed →
+  CompiledPolicy.compile p Γ = .ok cp →
+  ∃ wp,
+    wellTypedPolicy p Γ = .ok wp ∧
+    neverMatchesOpt? cp = neverMatches? wp (SymEnv.ofTypeEnv Γ)
+:= by
+  simp [neverMatches?, neverMatchesOpt?]
+  simp [sat?]
+  intro hwf h₀
+  have ⟨wp, h₁⟩ := compile_ok_then_exists_wtp hwf h₀
+  exists wp ; apply And.intro h₁
+  have ⟨asserts, h₂⟩ := verifyNeverMatches_is_ok hwf h₁
+  simp [h₂]
+  simp [cp_compile_produces_the_right_env h₀]
+  simp [compiled_policy_eq_wtp h₀ h₁]
+  have := verifyNeverMatchesOpt_eqv_verifyNeverMatches_ok h₀ h₁
+  simp [h₂, ResultAssertsEquiv] at this
+  exact Asserts.Equiv.satAsserts? [wp] _ (Asserts.Equiv.symm this)
+
+/--
+Full equivalence for `neverErrors?` and `neverErrorsOpt?`, including both the
+`.ok` and `.error` cases
+-/
+theorem neverErrorsOpt?_eqv_neverErrors? {p : Policy} {Γ : Validation.TypeEnv} :
+  Γ.WellFormed →
+  (do
+    let cp ← CompiledPolicy.compile p Γ
+    pure $ neverErrorsOpt? cp
+  ) =
+  (do
+    let wp ← wellTypedPolicy p Γ |>.mapError .validationError
+    pure $ neverErrors? wp (SymEnv.ofTypeEnv Γ)
+  )
+:= by
+  cases hcp : CompiledPolicy.compile p Γ
+  case ok cp =>
+    intro hwf
+    have ⟨wp, hwp, h⟩ := neverErrorsOpt?_eqv_neverErrors?_ok hwf hcp
+    simp [Except.mapError, hwp, h]
+  case error e =>
+    simp [Except.mapError]
+    cases hwp : wellTypedPolicy p Γ
+    case error e' =>
+      simp [CompiledPolicy.compile, Except.mapError, hwp] at hcp
+      simp [hcp]
+    case ok wp =>
+      intro hwf
+      have h := compile_ok_iff_welltypedpolicy_ok hwf (p := p)
+      simp [hcp, hwp, Except.isOk, Except.toBool] at h
+
+/--
+Full equivalence for `alwaysMatches?` and `alwaysMatchesOpt?`, including both the
+`.ok` and `.error` cases
+-/
+theorem alwaysMatchesOpt?_eqv_alwaysMatches? {p : Policy} {Γ : Validation.TypeEnv} :
+  Γ.WellFormed →
+  (do
+    let cp ← CompiledPolicy.compile p Γ
+    pure $ alwaysMatchesOpt? cp
+  ) =
+  (do
+    let wp ← wellTypedPolicy p Γ |>.mapError .validationError
+    pure $ alwaysMatches? wp (SymEnv.ofTypeEnv Γ)
+  )
+:= by
+  cases hcp : CompiledPolicy.compile p Γ
+  case ok cp =>
+    intro hwf
+    have ⟨wp, hwp, h⟩ := alwaysMatchesOpt?_eqv_alwaysMatches?_ok hwf hcp
+    simp [Except.mapError, hwp, h]
+  case error e =>
+    simp [Except.mapError]
+    cases hwp : wellTypedPolicy p Γ
+    case error e' =>
+      simp [CompiledPolicy.compile, Except.mapError, hwp] at hcp
+      simp [hcp]
+    case ok wp =>
+      intro hwf
+      have h := compile_ok_iff_welltypedpolicy_ok hwf (p := p)
+      simp [hcp, hwp, Except.isOk, Except.toBool] at h
+
+/--
+Full equivalence for `neverMatches?` and `neverMatchesOpt?`, including both the
+`.ok` and `.error` cases
+-/
+theorem neverMatchesOpt?_eqv_neverMatches? {p : Policy} {Γ : Validation.TypeEnv} :
+  Γ.WellFormed →
+  (do
+    let cp ← CompiledPolicy.compile p Γ
+    pure $ neverMatchesOpt? cp
+  ) =
+  (do
+    let wp ← wellTypedPolicy p Γ |>.mapError .validationError
+    pure $ neverMatches? wp (SymEnv.ofTypeEnv Γ)
+  )
+:= by
+  cases hcp : CompiledPolicy.compile p Γ
+  case ok cp =>
+    intro hwf
+    have ⟨wp, hwp, h⟩ := neverMatchesOpt?_eqv_neverMatches?_ok hwf hcp
+    simp [Except.mapError, hwp, h]
+  case error e =>
+    simp [Except.mapError]
+    cases hwp : wellTypedPolicy p Γ
+    case error e' =>
+      simp [CompiledPolicy.compile, Except.mapError, hwp] at hcp
+      simp [hcp]
+    case ok wp =>
+      intro hwf
+      have h := compile_ok_iff_welltypedpolicy_ok hwf (p := p)
+      simp [hcp, hwp, Except.isOk, Except.toBool] at h
+
+/--
+This theorem covers the "happy path" -- showing that if optimized policy
+compilation succeeds, then `wellTypedPolicies` succeeds and `implies?` and
+`impliesOpt?` are equivalent.
+-/
+theorem impliesOpt?_eqv_implies?_ok {ps₁ ps₂ : Policies} {cps₁ cps₂ : CompiledPolicies} {Γ : Validation.TypeEnv} :
+  Γ.WellFormed →
+  CompiledPolicies.compile ps₁ Γ = .ok cps₁ →
+  CompiledPolicies.compile ps₂ Γ = .ok cps₂ →
+  ∃ wps₁ wps₂,
+    wellTypedPolicies ps₁ Γ = .ok wps₁ ∧
+    wellTypedPolicies ps₂ Γ = .ok wps₂ ∧
+    impliesOpt? cps₁ cps₂ = implies? wps₁ wps₂ (SymEnv.ofTypeEnv Γ)
+:= by
+  simp [implies?, impliesOpt?]
+  simp [sat?]
+  intro hwf hcps₁ hcps₂
+  have ⟨wps₁, hwps₁⟩ := compile_ok_then_exists_wtps hwf hcps₁
+  exists wps₁ ; apply And.intro hwps₁
+  have ⟨wps₂, hwps₂⟩ := compile_ok_then_exists_wtps hwf hcps₂
+  exists wps₂ ; apply And.intro hwps₂
+  have ⟨asserts, h₁⟩ := verifyImplies_is_ok hwf hwps₁ hwps₂
+  simp [h₁]
+  simp [cps_compile_produces_the_right_env hcps₁]
+  simp [compiled_policies_eq_wtps hcps₁ hwps₁, compiled_policies_eq_wtps hcps₂ hwps₂]
+  have := verifyImpliesOpt_eqv_verifyImplies_ok hcps₁ hcps₂ hwps₁ hwps₂
+  simp [h₁, ResultAssertsEquiv] at this
+  exact Asserts.Equiv.satAsserts? _ _ (Asserts.Equiv.symm this)
+
+/--
+Full equivalence for `implies?` and `impliesOpt?`, including both the
+`.ok` and `.error` cases
+-/
+theorem impliesOpt?_eqv_implies? {ps₁ ps₂ : Policies} {Γ : Validation.TypeEnv} :
+  Γ.WellFormed →
+  (do
+    let cps₁ ← CompiledPolicies.compile ps₁ Γ
+    let cps₂ ← CompiledPolicies.compile ps₂ Γ
+    pure $ impliesOpt? cps₁ cps₂
+  ) =
+  (do
+    let wps₁ ← wellTypedPolicies ps₁ Γ |>.mapError .validationError
+    let wps₂ ← wellTypedPolicies ps₂ Γ |>.mapError .validationError
+    pure $ implies? wps₁ wps₂ (SymEnv.ofTypeEnv Γ)
+  )
+:= by
+  intro hwf
+  have h₁ := compile_ok_iff_welltypedpolicies_ok hwf (ps := ps₁)
+  have h₂ := compile_ok_iff_welltypedpolicies_ok hwf (ps := ps₂)
+  cases hcps₁ : CompiledPolicies.compile ps₁ Γ
+  <;> cases hcps₂ : CompiledPolicies.compile ps₂ Γ
+  <;> cases hwps₁ : wellTypedPolicies ps₁ Γ
+  <;> cases hwps₂ : wellTypedPolicies ps₂ Γ
+  -- this eliminates all the cases where the behavior of CompiledPolicies.compile is inconsistent
+  -- with the behavior of wellTypedPolicies on the same policyset
+  <;> simp_all [Except.mapError, Except.isOk, Except.toBool]
+  case ok.ok.ok.ok cps₁ cps₂ wps₁ wps₂ =>
+    have ⟨wps₁', wps₂', hwps₁', hwps₂', h⟩ := impliesOpt?_eqv_implies?_ok hwf hcps₁ hcps₂
+    simp_all
+  case error.ok.error.ok | error.error.error.error =>
+    simp [CompiledPolicies.compile, Except.mapError, hwps₁] at hcps₁
+    simp [hcps₁]
+  case ok.error.ok.error =>
+    simp [CompiledPolicies.compile, Except.mapError, hwps₂] at hcps₂
+    simp [hcps₂]
+
+/--
+This theorem covers the "happy path" -- showing that if optimized policy
+compilation succeeds, then `wellTypedPolicies` succeeds and `alwaysAllows?` and
+`alwaysAllowsOpt?` are equivalent.
+-/
+theorem alwaysAllowsOpt?_eqv_alwaysAllows?_ok {ps : Policies} {cps : CompiledPolicies} {Γ : Validation.TypeEnv} :
+  Γ.WellFormed →
+  CompiledPolicies.compile ps Γ = .ok cps →
+  ∃ wps,
+    wellTypedPolicies ps Γ = .ok wps ∧
+    alwaysAllowsOpt? cps = alwaysAllows? wps (SymEnv.ofTypeEnv Γ)
+:= by
+  simp [alwaysAllows?, alwaysAllowsOpt?]
+  simp [sat?]
+  intro hwf hcps
+  have ⟨wps, hwps⟩ := compile_ok_then_exists_wtps hwf hcps
+  exists wps ; apply And.intro hwps
+  have ⟨asserts, h₁⟩ := verifyAlwaysAllows_is_ok hwf hwps
+  simp [h₁]
+  simp [cps_compile_produces_the_right_env hcps]
+  simp [compiled_policies_eq_wtps hcps hwps]
+  have := verifyAlwaysAllowsOpt_eqv_verifyAlwaysAllows_ok hcps hwps
+  simp [h₁, ResultAssertsEquiv] at this
+  exact Asserts.Equiv.satAsserts? _ _ (Asserts.Equiv.symm this)
+
+/--
+Full equivalence for `alwaysAllows?` and `alwaysAllowsOpt?`, including both the
+`.ok` and `.error` cases
+-/
+theorem alwaysAllowsOpt?_eqv_alwaysAllows? {ps : Policies} {Γ : Validation.TypeEnv} :
+  Γ.WellFormed →
+  (do
+    let cps ← CompiledPolicies.compile ps Γ
+    pure $ alwaysAllowsOpt? cps
+  ) =
+  (do
+    let wps ← wellTypedPolicies ps Γ |>.mapError .validationError
+    pure $ alwaysAllows? wps (SymEnv.ofTypeEnv Γ)
+  )
+:= by
+  intro hwf
+  have h₁ := compile_ok_iff_welltypedpolicies_ok hwf (ps := ps)
+  cases hcps : CompiledPolicies.compile ps Γ
+  <;> cases hwps : wellTypedPolicies ps Γ
+  -- this eliminates all the cases where the behavior of CompiledPolicies.compile is inconsistent
+  -- with the behavior of wellTypedPolicies on the same policyset
+  <;> simp_all [Except.mapError, Except.isOk, Except.toBool]
+  case ok.ok cps wps =>
+    have ⟨wps', hwps', h⟩ := alwaysAllowsOpt?_eqv_alwaysAllows?_ok hwf hcps
+    simp_all
+  case error.error =>
+    simp [CompiledPolicies.compile, Except.mapError, hwps] at hcps
+    simp [hcps]
+
+/--
+This theorem covers the "happy path" -- showing that if optimized policy
+compilation succeeds, then `wellTypedPolicies` succeeds and `alwaysDenies?` and
+`alwaysDeniesOpt?` are equivalent.
+-/
+theorem alwaysDeniesOpt?_eqv_alwaysDenies?_ok {ps : Policies} {cps : CompiledPolicies} {Γ : Validation.TypeEnv} :
+  Γ.WellFormed →
+  CompiledPolicies.compile ps Γ = .ok cps →
+  ∃ wps,
+    wellTypedPolicies ps Γ = .ok wps ∧
+    alwaysDeniesOpt? cps = alwaysDenies? wps (SymEnv.ofTypeEnv Γ)
+:= by
+  simp [alwaysDenies?, alwaysDeniesOpt?]
+  simp [sat?]
+  intro hwf hcps
+  have ⟨wps, hwps⟩ := compile_ok_then_exists_wtps hwf hcps
+  exists wps ; apply And.intro hwps
+  have ⟨asserts, h₁⟩ := verifyAlwaysDenies_is_ok hwf hwps
+  simp [h₁]
+  simp [cps_compile_produces_the_right_env hcps]
+  simp [compiled_policies_eq_wtps hcps hwps]
+  have := verifyAlwaysDeniesOpt_eqv_verifyAlwaysDenies_ok hcps hwps
+  simp [h₁, ResultAssertsEquiv] at this
+  exact Asserts.Equiv.satAsserts? _ _ (Asserts.Equiv.symm this)
+
+/--
+Full equivalence for `alwaysDenies?` and `alwaysDeniesOpt?`, including both the
+`.ok` and `.error` cases
+-/
+theorem alwaysDeniesOpt?_eqv_alwaysDenies? {ps : Policies} {Γ : Validation.TypeEnv} :
+  Γ.WellFormed →
+  (do
+    let cps ← CompiledPolicies.compile ps Γ
+    pure $ alwaysDeniesOpt? cps
+  ) =
+  (do
+    let wps ← wellTypedPolicies ps Γ |>.mapError .validationError
+    pure $ alwaysDenies? wps (SymEnv.ofTypeEnv Γ)
+  )
+:= by
+  intro hwf
+  have h₁ := compile_ok_iff_welltypedpolicies_ok hwf (ps := ps)
+  cases hcps : CompiledPolicies.compile ps Γ
+  <;> cases hwps : wellTypedPolicies ps Γ
+  -- this eliminates all the cases where the behavior of CompiledPolicies.compile is inconsistent
+  -- with the behavior of wellTypedPolicies on the same policyset
+  <;> simp_all [Except.mapError, Except.isOk, Except.toBool]
+  case ok.ok cps wps =>
+    have ⟨wps', hwps', h⟩ := alwaysDeniesOpt?_eqv_alwaysDenies?_ok hwf hcps
+    simp_all
+  case error.error =>
+    simp [CompiledPolicies.compile, Except.mapError, hwps] at hcps
+    simp [hcps]
+
+/--
+This theorem covers the "happy path" -- showing that if optimized policy
+compilation succeeds, then `wellTypedPolicies` succeeds and `equivalent?` and
+`equivalentOpt?` are equivalent.
+-/
+theorem equivalentOpt?_eqv_equivalent?_ok {ps₁ ps₂ : Policies} {cps₁ cps₂ : CompiledPolicies} {Γ : Validation.TypeEnv} :
+  Γ.WellFormed →
+  CompiledPolicies.compile ps₁ Γ = .ok cps₁ →
+  CompiledPolicies.compile ps₂ Γ = .ok cps₂ →
+  ∃ wps₁ wps₂,
+    wellTypedPolicies ps₁ Γ = .ok wps₁ ∧
+    wellTypedPolicies ps₂ Γ = .ok wps₂ ∧
+    equivalentOpt? cps₁ cps₂ = equivalent? wps₁ wps₂ (SymEnv.ofTypeEnv Γ)
+:= by
+  simp [equivalent?, equivalentOpt?]
+  simp [sat?]
+  intro hwf hcps₁ hcps₂
+  have ⟨wps₁, hwps₁⟩ := compile_ok_then_exists_wtps hwf hcps₁
+  exists wps₁ ; apply And.intro hwps₁
+  have ⟨wps₂, hwps₂⟩ := compile_ok_then_exists_wtps hwf hcps₂
+  exists wps₂ ; apply And.intro hwps₂
+  have ⟨asserts, h₁⟩ := verifyEquivalent_is_ok hwf hwps₁ hwps₂
+  simp [h₁]
+  simp [cps_compile_produces_the_right_env hcps₁]
+  simp [compiled_policies_eq_wtps hcps₁ hwps₁, compiled_policies_eq_wtps hcps₂ hwps₂]
+  have := verifyEquivalentOpt_eqv_verifyEquivalent_ok hcps₁ hcps₂ hwps₁ hwps₂
+  simp [h₁, ResultAssertsEquiv] at this
+  exact Asserts.Equiv.satAsserts? _ _ (Asserts.Equiv.symm this)
+
+/--
+Full equivalence for `equivalent?` and `equivalentOpt?`, including both the
+`.ok` and `.error` cases
+-/
+theorem equivalentOpt?_eqv_equivalent? {ps₁ ps₂ : Policies} {Γ : Validation.TypeEnv} :
+  Γ.WellFormed →
+  (do
+    let cps₁ ← CompiledPolicies.compile ps₁ Γ
+    let cps₂ ← CompiledPolicies.compile ps₂ Γ
+    pure $ equivalentOpt? cps₁ cps₂
+  ) =
+  (do
+    let wps₁ ← wellTypedPolicies ps₁ Γ |>.mapError .validationError
+    let wps₂ ← wellTypedPolicies ps₂ Γ |>.mapError .validationError
+    pure $ equivalent? wps₁ wps₂ (SymEnv.ofTypeEnv Γ)
+  )
+:= by
+  intro hwf
+  have h₁ := compile_ok_iff_welltypedpolicies_ok hwf (ps := ps₁)
+  have h₂ := compile_ok_iff_welltypedpolicies_ok hwf (ps := ps₂)
+  cases hcps₁ : CompiledPolicies.compile ps₁ Γ
+  <;> cases hcps₂ : CompiledPolicies.compile ps₂ Γ
+  <;> cases hwps₁ : wellTypedPolicies ps₁ Γ
+  <;> cases hwps₂ : wellTypedPolicies ps₂ Γ
+  -- this eliminates all the cases where the behavior of CompiledPolicies.compile is inconsistent
+  -- with the behavior of wellTypedPolicies on the same policyset
+  <;> simp_all [Except.mapError, Except.isOk, Except.toBool]
+  case ok.ok.ok.ok cps₁ cps₂ wps₁ wps₂ =>
+    have ⟨wps₁', wps₂', hwps₁', hwps₂', h⟩ := equivalentOpt?_eqv_equivalent?_ok hwf hcps₁ hcps₂
+    simp_all
+  case error.ok.error.ok | error.error.error.error =>
+    simp [CompiledPolicies.compile, Except.mapError, hwps₁] at hcps₁
+    simp [hcps₁]
+  case ok.error.ok.error =>
+    simp [CompiledPolicies.compile, Except.mapError, hwps₂] at hcps₂
+    simp [hcps₂]
+
+/--
+This theorem covers the "happy path" -- showing that if optimized policy
+compilation succeeds, then `wellTypedPolicies` succeeds and `disjoint?` and
+`disjointOpt?` are equivalent.
+-/
+theorem disjointOpt?_eqv_disjoint?_ok {ps₁ ps₂ : Policies} {cps₁ cps₂ : CompiledPolicies} {Γ : Validation.TypeEnv} :
+  Γ.WellFormed →
+  CompiledPolicies.compile ps₁ Γ = .ok cps₁ →
+  CompiledPolicies.compile ps₂ Γ = .ok cps₂ →
+  ∃ wps₁ wps₂,
+    wellTypedPolicies ps₁ Γ = .ok wps₁ ∧
+    wellTypedPolicies ps₂ Γ = .ok wps₂ ∧
+    disjointOpt? cps₁ cps₂ = disjoint? wps₁ wps₂ (SymEnv.ofTypeEnv Γ)
+:= by
+  simp [disjoint?, disjointOpt?]
+  simp [sat?]
+  intro hwf hcps₁ hcps₂
+  have ⟨wps₁, hwps₁⟩ := compile_ok_then_exists_wtps hwf hcps₁
+  exists wps₁ ; apply And.intro hwps₁
+  have ⟨wps₂, hwps₂⟩ := compile_ok_then_exists_wtps hwf hcps₂
+  exists wps₂ ; apply And.intro hwps₂
+  have ⟨asserts, h₁⟩ := verifyDisjoint_is_ok hwf hwps₁ hwps₂
+  simp [h₁]
+  simp [cps_compile_produces_the_right_env hcps₁]
+  simp [compiled_policies_eq_wtps hcps₁ hwps₁, compiled_policies_eq_wtps hcps₂ hwps₂]
+  have := verifyDisjointOpt_eqv_verifyDisjoint_ok hcps₁ hcps₂ hwps₁ hwps₂
+  simp [h₁, ResultAssertsEquiv] at this
+  exact Asserts.Equiv.satAsserts? _ _ (Asserts.Equiv.symm this)
+
+/--
+Full equivalence for `disjoint?` and `disjointOpt?`, including both the
+`.ok` and `.error` cases
+-/
+theorem disjointOpt?_eqv_disjoint? {ps₁ ps₂ : Policies} {Γ : Validation.TypeEnv} :
+  Γ.WellFormed →
+  (do
+    let cps₁ ← CompiledPolicies.compile ps₁ Γ
+    let cps₂ ← CompiledPolicies.compile ps₂ Γ
+    pure $ disjointOpt? cps₁ cps₂
+  ) =
+  (do
+    let wps₁ ← wellTypedPolicies ps₁ Γ |>.mapError .validationError
+    let wps₂ ← wellTypedPolicies ps₂ Γ |>.mapError .validationError
+    pure $ disjoint? wps₁ wps₂ (SymEnv.ofTypeEnv Γ)
+  )
+:= by
+  intro hwf
+  have h₁ := compile_ok_iff_welltypedpolicies_ok hwf (ps := ps₁)
+  have h₂ := compile_ok_iff_welltypedpolicies_ok hwf (ps := ps₂)
+  cases hcps₁ : CompiledPolicies.compile ps₁ Γ
+  <;> cases hcps₂ : CompiledPolicies.compile ps₂ Γ
+  <;> cases hwps₁ : wellTypedPolicies ps₁ Γ
+  <;> cases hwps₂ : wellTypedPolicies ps₂ Γ
+  -- this eliminates all the cases where the behavior of CompiledPolicies.compile is inconsistent
+  -- with the behavior of wellTypedPolicies on the same policyset
+  <;> simp_all [Except.mapError, Except.isOk, Except.toBool]
+  case ok.ok.ok.ok cps₁ cps₂ wps₁ wps₂ =>
+    have ⟨wps₁', wps₂', hwps₁', hwps₂', h⟩ := disjointOpt?_eqv_disjoint?_ok hwf hcps₁ hcps₂
+    simp_all
+  case error.ok.error.ok | error.error.error.error =>
+    simp [CompiledPolicies.compile, Except.mapError, hwps₁] at hcps₁
+    simp [hcps₁]
+  case ok.error.ok.error =>
+    simp [CompiledPolicies.compile, Except.mapError, hwps₂] at hcps₂
+    simp [hcps₂]
+
+/--
+This theorem covers the "happy path" -- showing that if optimized policy
+compilation succeeds, then `wellTypedPolicies` succeeds and `checkNeverErrors` and
+`checkNeverErrorsOpt?` are equivalent.
+-/
+theorem checkNeverErrorsOpt_eqv_checkNeverErrors_ok {p : Policy} {cp : CompiledPolicy} {Γ : Validation.TypeEnv} :
+  Γ.WellFormed →
+  CompiledPolicy.compile p Γ = .ok cp →
+  ∃ wp,
+    wellTypedPolicy p Γ = .ok wp ∧
+    checkNeverErrorsOpt cp = checkNeverErrors wp (SymEnv.ofTypeEnv Γ)
+:= by
+  simp [checkNeverErrors, checkNeverErrorsOpt]
+  simp [checkUnsat]
+  intro hwf h₀
+  have ⟨wp, h₁⟩ := compile_ok_then_exists_wtp hwf h₀
+  exists wp ; apply And.intro h₁
+  have ⟨asserts, h₂⟩ := verifyNeverErrors_is_ok hwf h₁
+  simp [h₂]
+  simp [cp_compile_produces_the_right_env h₀]
+  have := verifyNeverErrorsOpt_eqv_verifyNeverErrors_ok h₀ h₁
+  simp [h₂, ResultAssertsEquiv] at this
+  exact Asserts.Equiv.checkUnsatAsserts (Asserts.Equiv.symm this)
+
+/--
+This theorem covers the "happy path" -- showing that if optimized policy
+compilation succeeds, then `wellTypedPolicy` succeeds and `checkAlwaysMatches` and
+`checkAlwaysMatchesOpt` are equivalent.
+-/
+theorem checkAlwaysMatchesOpt_eqv_checkAlwaysMatches_ok {p : Policy} {cp : CompiledPolicy} {Γ : Validation.TypeEnv} :
+  Γ.WellFormed →
+  CompiledPolicy.compile p Γ = .ok cp →
+  ∃ wp,
+    wellTypedPolicy p Γ = .ok wp ∧
+    checkAlwaysMatchesOpt cp = checkAlwaysMatches wp (SymEnv.ofTypeEnv Γ)
+:= by
+  simp [checkAlwaysMatches, checkAlwaysMatchesOpt]
+  simp [checkUnsat]
+  intro hwf h₀
+  have ⟨wp, h₁⟩ := compile_ok_then_exists_wtp hwf h₀
+  exists wp ; apply And.intro h₁
+  have ⟨asserts, h₂⟩ := verifyAlwaysMatches_is_ok hwf h₁
+  simp [h₂]
+  simp [cp_compile_produces_the_right_env h₀]
+  have := verifyAlwaysMatchesOpt_eqv_verifyAlwaysMatches_ok h₀ h₁
+  simp [h₂, ResultAssertsEquiv] at this
+  exact Asserts.Equiv.checkUnsatAsserts (Asserts.Equiv.symm this)
+
+/--
+This theorem covers the "happy path" -- showing that if optimized policy
+compilation succeeds, then `wellTypedPolicy` succeeds and `checkNeverMatches` and
+`checkNeverMatchesOpt` are equivalent.
+-/
+theorem checkNeverMatchesOpt_eqv_checkNeverMatches_ok {p : Policy} {cp : CompiledPolicy} {Γ : Validation.TypeEnv} :
+  Γ.WellFormed →
+  CompiledPolicy.compile p Γ = .ok cp →
+  ∃ wp,
+    wellTypedPolicy p Γ = .ok wp ∧
+    checkNeverMatchesOpt cp = checkNeverMatches wp (SymEnv.ofTypeEnv Γ)
+:= by
+  simp [checkNeverMatches, checkNeverMatchesOpt]
+  simp [checkUnsat]
+  intro hwf h₀
+  have ⟨wp, h₁⟩ := compile_ok_then_exists_wtp hwf h₀
+  exists wp ; apply And.intro h₁
+  have ⟨asserts, h₂⟩ := verifyNeverMatches_is_ok hwf h₁
+  simp [h₂]
+  simp [cp_compile_produces_the_right_env h₀]
+  have := verifyNeverMatchesOpt_eqv_verifyNeverMatches_ok h₀ h₁
+  simp [h₂, ResultAssertsEquiv] at this
+  exact Asserts.Equiv.checkUnsatAsserts (Asserts.Equiv.symm this)
+
+/--
+Full equivalence for checkNeverErrors` and `checkNeverErrorsOpt`, including both the
+`.ok` and `.error` cases
+-/
+theorem checkNeverErrorsOpt_eqv_checkNeverErrors {p : Policy} {Γ : Validation.TypeEnv} :
+  Γ.WellFormed →
+  (do
+    let cp ← CompiledPolicy.compile p Γ
+    pure $ checkNeverErrorsOpt cp
+  ) =
+  (do
+    let wp ← wellTypedPolicy p Γ |>.mapError .validationError
+    pure $ checkNeverErrors wp (SymEnv.ofTypeEnv Γ)
+  )
+:= by
+  cases hcp : CompiledPolicy.compile p Γ
+  case ok cp =>
+    intro hwf
+    have ⟨wp, hwp, h⟩ := checkNeverErrorsOpt_eqv_checkNeverErrors_ok hwf hcp
+    simp [Except.mapError, hwp, h]
+  case error e =>
+    simp [Except.mapError]
+    cases hwp : wellTypedPolicy p Γ
+    case error e' =>
+      simp [CompiledPolicy.compile, Except.mapError, hwp] at hcp
+      simp [hcp]
+    case ok wp =>
+      intro hwf
+      have h := compile_ok_iff_welltypedpolicy_ok hwf (p := p)
+      simp [hcp, hwp, Except.isOk, Except.toBool] at h
+
+/--
+Full equivalence for `checkAlwaysMatches` and `checkAlwaysMatchesOpt`, including both the
+`.ok` and `.error` cases
+-/
+theorem checkAlwaysMatchesOpt_eqv_checkAlwaysMatches {p : Policy} {Γ : Validation.TypeEnv} :
+  Γ.WellFormed →
+  (do
+    let cp ← CompiledPolicy.compile p Γ
+    pure $ checkAlwaysMatchesOpt cp
+  ) =
+  (do
+    let wp ← wellTypedPolicy p Γ |>.mapError .validationError
+    pure $ checkAlwaysMatches wp (SymEnv.ofTypeEnv Γ)
+  )
+:= by
+  cases hcp : CompiledPolicy.compile p Γ
+  case ok cp =>
+    intro hwf
+    have ⟨wp, hwp, h⟩ := checkAlwaysMatchesOpt_eqv_checkAlwaysMatches_ok hwf hcp
+    simp [Except.mapError, hwp, h]
+  case error e =>
+    simp [Except.mapError]
+    cases hwp : wellTypedPolicy p Γ
+    case error e' =>
+      simp [CompiledPolicy.compile, Except.mapError, hwp] at hcp
+      simp [hcp]
+    case ok wp =>
+      intro hwf
+      have h := compile_ok_iff_welltypedpolicy_ok hwf (p := p)
+      simp [hcp, hwp, Except.isOk, Except.toBool] at h
+
+/--
+Full equivalence for `checkNeverMatches` and `checkNeverMatchesOpt`, including both the
+`.ok` and `.error` cases
+-/
+theorem checkNeverMatchesOpt_eqv_checkNeverMatches {p : Policy} {Γ : Validation.TypeEnv} :
+  Γ.WellFormed →
+  (do
+    let cp ← CompiledPolicy.compile p Γ
+    pure $ checkNeverMatchesOpt cp
+  ) =
+  (do
+    let wp ← wellTypedPolicy p Γ |>.mapError .validationError
+    pure $ checkNeverMatches wp (SymEnv.ofTypeEnv Γ)
+  )
+:= by
+  cases hcp : CompiledPolicy.compile p Γ
+  case ok cp =>
+    intro hwf
+    have ⟨wp, hwp, h⟩ := checkNeverMatchesOpt_eqv_checkNeverMatches_ok hwf hcp
+    simp [Except.mapError, hwp, h]
+  case error e =>
+    simp [Except.mapError]
+    cases hwp : wellTypedPolicy p Γ
+    case error e' =>
+      simp [CompiledPolicy.compile, Except.mapError, hwp] at hcp
+      simp [hcp]
+    case ok wp =>
+      intro hwf
+      have h := compile_ok_iff_welltypedpolicy_ok hwf (p := p)
+      simp [hcp, hwp, Except.isOk, Except.toBool] at h
+
+/--
+This theorem covers the "happy path" -- showing that if optimized policy
+compilation succeeds, then `wellTypedPolicies` succeeds and `checkImplies` and
+`checkImpliesOpt` are equivalent.
+-/
+theorem checkImpliesOpt_eqv_checkImplies_ok {ps₁ ps₂ : Policies} {cps₁ cps₂ : CompiledPolicies} {Γ : Validation.TypeEnv} :
+  Γ.WellFormed →
+  CompiledPolicies.compile ps₁ Γ = .ok cps₁ →
+  CompiledPolicies.compile ps₂ Γ = .ok cps₂ →
+  ∃ wps₁ wps₂,
+    wellTypedPolicies ps₁ Γ = .ok wps₁ ∧
+    wellTypedPolicies ps₂ Γ = .ok wps₂ ∧
+    checkImpliesOpt cps₁ cps₂ = checkImplies wps₁ wps₂ (SymEnv.ofTypeEnv Γ)
+:= by
+  simp [checkImplies, checkImpliesOpt]
+  simp [checkUnsat]
+  intro hwf hcps₁ hcps₂
+  have ⟨wps₁, hwps₁⟩ := compile_ok_then_exists_wtps hwf hcps₁
+  exists wps₁ ; apply And.intro hwps₁
+  have ⟨wps₂, hwps₂⟩ := compile_ok_then_exists_wtps hwf hcps₂
+  exists wps₂ ; apply And.intro hwps₂
+  have ⟨asserts, h₁⟩ := verifyImplies_is_ok hwf hwps₁ hwps₂
+  simp [h₁]
+  simp [cps_compile_produces_the_right_env hcps₁]
+  have := verifyImpliesOpt_eqv_verifyImplies_ok hcps₁ hcps₂ hwps₁ hwps₂
+  simp [h₁, ResultAssertsEquiv] at this
+  exact Asserts.Equiv.checkUnsatAsserts (Asserts.Equiv.symm this)
+
+/--
+Full equivalence for `checkImplies` and `checkImpliesOpt`, including both the
+`.ok` and `.error` cases
+-/
+theorem checkImpliesOpt_eqv_checkImplies {ps₁ ps₂ : Policies} {Γ : Validation.TypeEnv} :
+  Γ.WellFormed →
+  (do
+    let cps₁ ← CompiledPolicies.compile ps₁ Γ
+    let cps₂ ← CompiledPolicies.compile ps₂ Γ
+    pure $ checkImpliesOpt cps₁ cps₂
+  ) =
+  (do
+    let wps₁ ← wellTypedPolicies ps₁ Γ |>.mapError .validationError
+    let wps₂ ← wellTypedPolicies ps₂ Γ |>.mapError .validationError
+    pure $ checkImplies wps₁ wps₂ (SymEnv.ofTypeEnv Γ)
+  )
+:= by
+  intro hwf
+  have h₁ := compile_ok_iff_welltypedpolicies_ok hwf (ps := ps₁)
+  have h₂ := compile_ok_iff_welltypedpolicies_ok hwf (ps := ps₂)
+  cases hcps₁ : CompiledPolicies.compile ps₁ Γ
+  <;> cases hcps₂ : CompiledPolicies.compile ps₂ Γ
+  <;> cases hwps₁ : wellTypedPolicies ps₁ Γ
+  <;> cases hwps₂ : wellTypedPolicies ps₂ Γ
+  -- this eliminates all the cases where the behavior of CompiledPolicies.compile is inconsistent
+  -- with the behavior of wellTypedPolicies on the same policyset
+  <;> simp_all [Except.mapError, Except.isOk, Except.toBool]
+  case ok.ok.ok.ok cps₁ cps₂ wps₁ wps₂ =>
+    have ⟨wps₁', wps₂', hwps₁', hwps₂', h⟩ := checkImpliesOpt_eqv_checkImplies_ok hwf hcps₁ hcps₂
+    simp_all
+  case error.ok.error.ok | error.error.error.error =>
+    simp [CompiledPolicies.compile, Except.mapError, hwps₁] at hcps₁
+    simp [hcps₁]
+  case ok.error.ok.error =>
+    simp [CompiledPolicies.compile, Except.mapError, hwps₂] at hcps₂
+    simp [hcps₂]
+
+/--
+This theorem covers the "happy path" -- showing that if optimized policy
+compilation succeeds, then `wellTypedPolicies` succeeds and `checkAlwaysAllows` and
+`checkAlwaysAllowsOpt` are equivalent.
+-/
+theorem checkAlwaysAllowsOpt_eqv_checkAlwaysAllows_ok {ps : Policies} {cps : CompiledPolicies} {Γ : Validation.TypeEnv} :
+  Γ.WellFormed →
+  CompiledPolicies.compile ps Γ = .ok cps →
+  ∃ wps,
+    wellTypedPolicies ps Γ = .ok wps ∧
+    checkAlwaysAllowsOpt cps = checkAlwaysAllows wps (SymEnv.ofTypeEnv Γ)
+:= by
+  simp [checkAlwaysAllows, checkAlwaysAllowsOpt]
+  simp [checkUnsat]
+  intro hwf hcps
+  have ⟨wps, hwps⟩ := compile_ok_then_exists_wtps hwf hcps
+  exists wps ; apply And.intro hwps
+  have ⟨asserts, h₁⟩ := verifyAlwaysAllows_is_ok hwf hwps
+  simp [h₁]
+  simp [cps_compile_produces_the_right_env hcps]
+  have := verifyAlwaysAllowsOpt_eqv_verifyAlwaysAllows_ok hcps hwps
+  simp [h₁, ResultAssertsEquiv] at this
+  exact Asserts.Equiv.checkUnsatAsserts (Asserts.Equiv.symm this)
+
+/--
+Full equivalence for `checkAlwaysAllows` and `checkAlwaysAllowsOpt`, including both the
+`.ok` and `.error` cases
+-/
+theorem checkAlwaysAllowsOpt_eqv_checkAlwaysAllows {ps : Policies} {Γ : Validation.TypeEnv} :
+  Γ.WellFormed →
+  (do
+    let cps ← CompiledPolicies.compile ps Γ
+    pure $ checkAlwaysAllowsOpt cps
+  ) =
+  (do
+    let wps ← wellTypedPolicies ps Γ |>.mapError .validationError
+    pure $ checkAlwaysAllows wps (SymEnv.ofTypeEnv Γ)
+  )
+:= by
+  intro hwf
+  have h₁ := compile_ok_iff_welltypedpolicies_ok hwf (ps := ps)
+  cases hcps : CompiledPolicies.compile ps Γ
+  <;> cases hwps : wellTypedPolicies ps Γ
+  -- this eliminates all the cases where the behavior of CompiledPolicies.compile is inconsistent
+  -- with the behavior of wellTypedPolicies on the same policyset
+  <;> simp_all [Except.mapError, Except.isOk, Except.toBool]
+  case ok.ok cps wps =>
+    have ⟨wps', hwps', h⟩ := checkAlwaysAllowsOpt_eqv_checkAlwaysAllows_ok hwf hcps
+    simp_all
+  case error.error =>
+    simp [CompiledPolicies.compile, Except.mapError, hwps] at hcps
+    simp [hcps]
+
+/--
+This theorem covers the "happy path" -- showing that if optimized policy
+compilation succeeds, then `wellTypedPolicies` succeeds and `checkAlwaysDenies` and
+`checkAlwaysDeniesOpt` are equivalent.
+-/
+theorem checkAlwaysDeniesOpt_eqv_checkAlwaysDenies_ok {ps : Policies} {cps : CompiledPolicies} {Γ : Validation.TypeEnv} :
+  Γ.WellFormed →
+  CompiledPolicies.compile ps Γ = .ok cps →
+  ∃ wps,
+    wellTypedPolicies ps Γ = .ok wps ∧
+    checkAlwaysDeniesOpt cps = checkAlwaysDenies wps (SymEnv.ofTypeEnv Γ)
+:= by
+  simp [checkAlwaysDenies, checkAlwaysDeniesOpt]
+  simp [checkUnsat]
+  intro hwf hcps
+  have ⟨wps, hwps⟩ := compile_ok_then_exists_wtps hwf hcps
+  exists wps ; apply And.intro hwps
+  have ⟨asserts, h₁⟩ := verifyAlwaysDenies_is_ok hwf hwps
+  simp [h₁]
+  simp [cps_compile_produces_the_right_env hcps]
+  have := verifyAlwaysDeniesOpt_eqv_verifyAlwaysDenies_ok hcps hwps
+  simp [h₁, ResultAssertsEquiv] at this
+  exact Asserts.Equiv.checkUnsatAsserts (Asserts.Equiv.symm this)
+
+/--
+Full equivalence for `checkAlwaysDenies` and `checkAlwaysDeniesOpt`, including both the
+`.ok` and `.error` cases
+-/
+theorem checkAlwaysDeniesOpt_eqv_checkAlwaysDenies {ps : Policies} {Γ : Validation.TypeEnv} :
+  Γ.WellFormed →
+  (do
+    let cps ← CompiledPolicies.compile ps Γ
+    pure $ checkAlwaysDeniesOpt cps
+  ) =
+  (do
+    let wps ← wellTypedPolicies ps Γ |>.mapError .validationError
+    pure $ checkAlwaysDenies wps (SymEnv.ofTypeEnv Γ)
+  )
+:= by
+  intro hwf
+  have h₁ := compile_ok_iff_welltypedpolicies_ok hwf (ps := ps)
+  cases hcps : CompiledPolicies.compile ps Γ
+  <;> cases hwps : wellTypedPolicies ps Γ
+  -- this eliminates all the cases where the behavior of CompiledPolicies.compile is inconsistent
+  -- with the behavior of wellTypedPolicies on the same policyset
+  <;> simp_all [Except.mapError, Except.isOk, Except.toBool]
+  case ok.ok cps wps =>
+    have ⟨wps', hwps', h⟩ := checkAlwaysDeniesOpt_eqv_checkAlwaysDenies_ok hwf hcps
+    simp_all
+  case error.error =>
+    simp [CompiledPolicies.compile, Except.mapError, hwps] at hcps
+    simp [hcps]
+
+/--
+This theorem covers the "happy path" -- showing that if optimized policy
+compilation succeeds, then `wellTypedPolicies` succeeds and `checkEquivalent` and
+`checkEquivalentOpt` are equivalent.
+-/
+theorem checkEquivalentOpt_eqv_checkEquivalent_ok {ps₁ ps₂ : Policies} {cps₁ cps₂ : CompiledPolicies} {Γ : Validation.TypeEnv} :
+  Γ.WellFormed →
+  CompiledPolicies.compile ps₁ Γ = .ok cps₁ →
+  CompiledPolicies.compile ps₂ Γ = .ok cps₂ →
+  ∃ wps₁ wps₂,
+    wellTypedPolicies ps₁ Γ = .ok wps₁ ∧
+    wellTypedPolicies ps₂ Γ = .ok wps₂ ∧
+    checkEquivalentOpt cps₁ cps₂ = checkEquivalent wps₁ wps₂ (SymEnv.ofTypeEnv Γ)
+:= by
+  simp [checkEquivalent, checkEquivalentOpt]
+  simp [checkUnsat]
+  intro hwf hcps₁ hcps₂
+  have ⟨wps₁, hwps₁⟩ := compile_ok_then_exists_wtps hwf hcps₁
+  exists wps₁ ; apply And.intro hwps₁
+  have ⟨wps₂, hwps₂⟩ := compile_ok_then_exists_wtps hwf hcps₂
+  exists wps₂ ; apply And.intro hwps₂
+  have ⟨asserts, h₁⟩ := verifyEquivalent_is_ok hwf hwps₁ hwps₂
+  simp [h₁]
+  simp [cps_compile_produces_the_right_env hcps₁]
+  have := verifyEquivalentOpt_eqv_verifyEquivalent_ok hcps₁ hcps₂ hwps₁ hwps₂
+  simp [h₁, ResultAssertsEquiv] at this
+  exact Asserts.Equiv.checkUnsatAsserts (Asserts.Equiv.symm this)
+
+/--
+Full equivalence for `checkEquivalent` and `checkEquivalentOpt`, including both the
+`.ok` and `.error` cases
+-/
+theorem checkEquivalentOpt_eqv_checkEquivalent {ps₁ ps₂ : Policies} {Γ : Validation.TypeEnv} :
+  Γ.WellFormed →
+  (do
+    let cps₁ ← CompiledPolicies.compile ps₁ Γ
+    let cps₂ ← CompiledPolicies.compile ps₂ Γ
+    pure $ checkEquivalentOpt cps₁ cps₂
+  ) =
+  (do
+    let wps₁ ← wellTypedPolicies ps₁ Γ |>.mapError .validationError
+    let wps₂ ← wellTypedPolicies ps₂ Γ |>.mapError .validationError
+    pure $ checkEquivalent wps₁ wps₂ (SymEnv.ofTypeEnv Γ)
+  )
+:= by
+  intro hwf
+  have h₁ := compile_ok_iff_welltypedpolicies_ok hwf (ps := ps₁)
+  have h₂ := compile_ok_iff_welltypedpolicies_ok hwf (ps := ps₂)
+  cases hcps₁ : CompiledPolicies.compile ps₁ Γ
+  <;> cases hcps₂ : CompiledPolicies.compile ps₂ Γ
+  <;> cases hwps₁ : wellTypedPolicies ps₁ Γ
+  <;> cases hwps₂ : wellTypedPolicies ps₂ Γ
+  -- this eliminates all the cases where the behavior of CompiledPolicies.compile is inconsistent
+  -- with the behavior of wellTypedPolicies on the same policyset
+  <;> simp_all [Except.mapError, Except.isOk, Except.toBool]
+  case ok.ok.ok.ok cps₁ cps₂ wps₁ wps₂ =>
+    have ⟨wps₁', wps₂', hwps₁', hwps₂', h⟩ := checkEquivalentOpt_eqv_checkEquivalent_ok hwf hcps₁ hcps₂
+    simp_all
+  case error.ok.error.ok | error.error.error.error =>
+    simp [CompiledPolicies.compile, Except.mapError, hwps₁] at hcps₁
+    simp [hcps₁]
+  case ok.error.ok.error =>
+    simp [CompiledPolicies.compile, Except.mapError, hwps₂] at hcps₂
+    simp [hcps₂]
+
+/--
+This theorem covers the "happy path" -- showing that if optimized policy
+compilation succeeds, then `wellTypedPolicies` succeeds and `checkDisjoint` and
+`checkDisjointOpt` are equivalent.
+-/
+theorem checkDisjointOpt_eqv_checkDisjoint_ok {ps₁ ps₂ : Policies} {cps₁ cps₂ : CompiledPolicies} {Γ : Validation.TypeEnv} :
+  Γ.WellFormed →
+  CompiledPolicies.compile ps₁ Γ = .ok cps₁ →
+  CompiledPolicies.compile ps₂ Γ = .ok cps₂ →
+  ∃ wps₁ wps₂,
+    wellTypedPolicies ps₁ Γ = .ok wps₁ ∧
+    wellTypedPolicies ps₂ Γ = .ok wps₂ ∧
+    checkDisjointOpt cps₁ cps₂ = checkDisjoint wps₁ wps₂ (SymEnv.ofTypeEnv Γ)
+:= by
+  simp [checkDisjoint, checkDisjointOpt]
+  simp [checkUnsat]
+  intro hwf hcps₁ hcps₂
+  have ⟨wps₁, hwps₁⟩ := compile_ok_then_exists_wtps hwf hcps₁
+  exists wps₁ ; apply And.intro hwps₁
+  have ⟨wps₂, hwps₂⟩ := compile_ok_then_exists_wtps hwf hcps₂
+  exists wps₂ ; apply And.intro hwps₂
+  have ⟨asserts, h₁⟩ := verifyDisjoint_is_ok hwf hwps₁ hwps₂
+  simp [h₁]
+  simp [cps_compile_produces_the_right_env hcps₁]
+  have := verifyDisjointOpt_eqv_verifyDisjoint_ok hcps₁ hcps₂ hwps₁ hwps₂
+  simp [h₁, ResultAssertsEquiv] at this
+  exact Asserts.Equiv.checkUnsatAsserts (Asserts.Equiv.symm this)
+
+/--
+Full equivalence for `checkDisjoint` and `checkDisjointOpt`, including both the
+`.ok` and `.error` cases
+-/
+theorem checkDisjointOpt_eqv_checkDisjoint {ps₁ ps₂ : Policies} {Γ : Validation.TypeEnv} :
+  Γ.WellFormed →
+  (do
+    let cps₁ ← CompiledPolicies.compile ps₁ Γ
+    let cps₂ ← CompiledPolicies.compile ps₂ Γ
+    pure $ checkDisjointOpt cps₁ cps₂
+  ) =
+  (do
+    let wps₁ ← wellTypedPolicies ps₁ Γ |>.mapError .validationError
+    let wps₂ ← wellTypedPolicies ps₂ Γ |>.mapError .validationError
+    pure $ checkDisjoint wps₁ wps₂ (SymEnv.ofTypeEnv Γ)
+  )
+:= by
+  intro hwf
+  have h₁ := compile_ok_iff_welltypedpolicies_ok hwf (ps := ps₁)
+  have h₂ := compile_ok_iff_welltypedpolicies_ok hwf (ps := ps₂)
+  cases hcps₁ : CompiledPolicies.compile ps₁ Γ
+  <;> cases hcps₂ : CompiledPolicies.compile ps₂ Γ
+  <;> cases hwps₁ : wellTypedPolicies ps₁ Γ
+  <;> cases hwps₂ : wellTypedPolicies ps₂ Γ
+  -- this eliminates all the cases where the behavior of CompiledPolicies.compile is inconsistent
+  -- with the behavior of wellTypedPolicies on the same policyset
+  <;> simp_all [Except.mapError, Except.isOk, Except.toBool]
+  case ok.ok.ok.ok cps₁ cps₂ wps₁ wps₂ =>
+    have ⟨wps₁', wps₂', hwps₁', hwps₂', h⟩ := checkDisjointOpt_eqv_checkDisjoint_ok hwf hcps₁ hcps₂
+    simp_all
+  case error.ok.error.ok | error.error.error.error =>
+    simp [CompiledPolicies.compile, Except.mapError, hwps₁] at hcps₁
+    simp [hcps₁]
+  case ok.error.ok.error =>
+    simp [CompiledPolicies.compile, Except.mapError, hwps₂] at hcps₂
+    simp [hcps₂]
